\textcolor{red}{
First, we isolate $f_L$ from the $f_0=\frac{1}{2}(f_L+f_U)$ expression:
\begin{equation*}
	2f_0=(f_L+f_U)\Rightarrow f_L=2f_0-f_U
\end{equation*}
Then we replace it in the expression of $Q$:
\begin{align*}
	Q&=\frac{f_0}{\Delta f}=\frac{f_0}{(f_U-f_L)}=\frac{f_0}{(f_U-2f_0+f_U)}=\frac{f_0}{2(f_U-f_0)}\Rightarrow 2(f_U-f_0)=\frac{f_0}{Q}\\
	&\Rightarrow 2f_U=\frac{f_0}{Q}+2f_0\Rightarrow f_U=f_0\left(1+\frac{1}{2Q}\right)
\end{align*}
Now, replacing $f_U$ into $\Delta f=f_U-f_L$ gives
\begin{equation*}
	f_L=f_U-\Delta f\Rightarrow f_L=f_U-\frac{f_0}{Q}
	\Rightarrow f_L=f_0\left(\frac{1}{2Q}+1\right)-\frac{f_0}{Q}=f_0\left(1-\frac{1}{2Q}\right)
\end{equation*}
}